\section{115 --- Distinct Subsequences}
Given a string $S$ and a string $T$, count the number of distinct subsequences of $S$ which equals $T$.
\par
A subsequence of a string is a new string which is formed from the original string by deleting some (can be none) of the characters without disturbing the relative positions of the remaining characters. (i.e, \texttt{ACE} is a subsequence of \texttt{ABCDE} while \texttt{AEC} is not).
\paragraph{Example 1:}
\begin{flushleft}
\textbf{Input}: $S = \texttt{rabbbit}$, $T = \texttt{rabbit}$
\\
\textbf{Output}: 3
\\
\textbf{Explanation}:
\\
As shown below, there are 3 ways you can generate \texttt{rabbit} from $S$.
\begin{itemize}
    \item \textbf{rabb}b\textbf{it}
    \item \textbf{ra}b\textbf{bbit}
    \item \textbf{rab}b\textbf{bit}
\end{itemize}
\end{flushleft}
\paragraph{Example 2:}
\begin{flushleft}
\textbf{Input}: $S = \texttt{babgbag}$,  $T = \texttt{bag}$
\\
\textbf{Output}: 5
\\
\textbf{Explanation}:
\\
As shown below, there are 5 ways you can generate \texttt{bag} from $S$.
\begin{itemize}
    \item \textbf{ba}b\textbf{g}bag
    \item \textbf{ba}bgba\textbf{g}
    \item \textbf{b}abgb\textbf{ag}
    \item ba\textbf{b}gb\textbf{ag}
    \item babg\textbf{bag}
    \end{itemize}
\end{flushleft}
\subsection{Dynamic Programming}
\begin{CJK*}{UTF8}{gbsn}
这种问题一般依靠Dynamic Programming来解决，假设$F[i][j]$表示$S[0,i-1]$中能够表示$T[0,j-1]$的subsequence的个数，$i=0$或者$j=0$则表示$S[0,-1]$或者$T[0,-1]$是空字符串。很显然$F[i][0]=1$因为对于$T$为空字符串，$S$中只有一个subsequence也就是空字符串能表示空字符串。对于$i>0$ and $j>0$，首先$F[i][j] = 0 + F[i-1][j]$即首先要加上$S[0,i-2]$中能够表示$T[0,j-1]$的subsequence的个数，接着看$S[i-1]$是否和$T[j-1]$相等，如果相等，$F[i][j]$还要加上$F[i-1][j-1]$，即$S[0,i-2]$中能够表示$T[0,j-2]$的subsequence的个数。不相等就不用加了。
\end{CJK*}
\setcounter{algorithm}{0}
\begin{algorithm}[H]
\caption{Dynamic Programming}
\begin{algorithmic}[1]
\Procedure{NumDistinct}{$S,\;L_S,\;T,\;L_T$}
\State Initialize DP array $F[i][j]$
\State $F[0][0]=\ldots=F[L_S+1][L_T+1]:=0$
\For{$x:=0 \to L_S$}
\State $F[x][0]\gets 1$ \Comment Empty string only has one way to represent
\EndFor
\For{$x:=1 \to L_S$}
\For{$y:=1 \to L_T$}
\State $F[x][y]\gets F[x-1][y]$ 
\If{$S[x-1]=T[y-1]$}
\State $F[x][y]\gets F[x][y] + F[x-1][y-1]$
\EndIf
\EndFor
\EndFor
\State \Return $F[L_S][L_T]$
\EndProcedure
\end{algorithmic}
\end{algorithm}

