\section{143 --- Reorder List}
Given a singly linked list $L$: 
\begin{figure}[H]
\begin{tikzpicture}
[mynode/.style={draw,circle,minimum size=10mm, fill=gray!20!}]
\node(){};
\node[mynode](0) {\scalebox{0.6}{$L_0$}};
\node[mynode](1)[right=15mm of 0] {\scalebox{0.6}{$L_1$}};
\node[mynode](2)[right=15mm of 1] {$\ldots$};
\node[mynode](n1)[right=15mm of 2] {\scalebox{0.6}{$L_{n-1}$}};
\node[mynode](n2)[right=15mm of n1] {\scalebox{0.6}{$L_n$}};
\draw[>=stealth,->] (0) -- (1);
\draw[>=stealth,->] (1) -- (2);
\draw[>=stealth,->] (2) -- (n1);
\draw[>=stealth,->] (n1) -- (n2);
\end{tikzpicture}
\end{figure}
reorder it to:
\begin{figure}[H]
\begin{tikzpicture}
[mynode/.style={draw,circle,minimum size=10mm, fill=gray!20!}]
\node(){};
\node[mynode](0) {\scalebox{0.6}{$L_0$}};
\node[mynode](n2)[right=15mm of 0] {\scalebox{0.6}{$L_n$}};
\node[mynode](1)[right=15mm of n2] {\scalebox{0.6}{$L_1$}};
\node[mynode](n1)[right=15mm of 1] {\scalebox{0.6}{$L_{n-1}$}};
\node[mynode](2)[right=15mm of n1] {$\ldots$};
\draw[>=stealth,->] (0) -- (n2);
\draw[>=stealth,->] (n2) -- (1);
\draw[>=stealth,->] (1) -- (n1);
\draw[>=stealth,->] (n1) -- (2);
\end{tikzpicture}
\end{figure}
You may \textbf{not} modify the values in the list's nodes, only nodes itself may be changed.
\paragraph{Example 1:}
\begin{flushleft}
Given:
\begin{figure}[H]
\begin{tikzpicture}
[mynode/.style={draw,circle,minimum size=5mm, fill=gray!20!}]
\node(){};
\node[mynode](1) {1};
\node[mynode](2)[right=8mm of 1] {2};
\node[mynode](3)[right=8mm of 2] {3};
\node[mynode](4)[right=8mm of 3] {4};
\draw[>=stealth,->] (1) -- (2);
\draw[>=stealth,->] (2) -- (3);
\draw[>=stealth,->] (3) -- (4);
\end{tikzpicture}
\end{figure}
Reorder to:
\begin{figure}[H]
\begin{tikzpicture}
[mynode/.style={draw,circle,minimum size=5mm, fill=gray!20!}]
\node(){};
\node[mynode](1) {1};
\node[mynode](4)[right=8mm of 1] {4};
\node[mynode](2)[right=8mm of 4] {2};
\node[mynode](3)[right=8mm of 2] {3};
\draw[>=stealth,->] (1) -- (4);
\draw[>=stealth,->] (4) -- (2);
\draw[>=stealth,->] (2) -- (3);
\end{tikzpicture}
\end{figure}
\end{flushleft}
\paragraph{Example 2:}
\begin{flushleft}
Given:
\begin{figure}[H]
\begin{tikzpicture}
[mynode/.style={draw,circle,minimum size=5mm, fill=gray!20!}]
\node(){};
\node[mynode](1) {1};
\node[mynode](2)[right=8mm of 1] {2};
\node[mynode](3)[right=8mm of 2] {3};
\node[mynode](4)[right=8mm of 3] {4};
\node[mynode](5)[right=8mm of 4] {5};
\draw[>=stealth,->] (1) -- (2);
\draw[>=stealth,->] (2) -- (3);
\draw[>=stealth,->] (3) -- (4);
\draw[>=stealth,->] (4) -- (5);
\end{tikzpicture}
\end{figure}
Reorder to:
\begin{figure}[H]
\begin{tikzpicture}
[mynode/.style={draw,circle,minimum size=5mm, fill=gray!20!}]
\node(){};
\node[mynode](1) {1};
\node[mynode](5)[right=8mm of 1] {5};
\node[mynode](2)[right=8mm of 5] {2};
\node[mynode](4)[right=8mm of 2] {4};
\node[mynode](3)[right=8mm of 4] {3};
\draw[>=stealth,->] (1) -- (5);
\draw[>=stealth,->] (5) -- (2);
\draw[>=stealth,->] (2) -- (4);
\draw[>=stealth,->] (4) -- (3);
\end{tikzpicture}
\end{figure}
\end{flushleft}
\subsection{Two Pointers + Reverse}
首先用快慢指针找到链表的中间位置的node，然后从这个位置，将这个链表断开。然后对后半部分的链表进行reverse操作，最后合并两个链表。
\setcounter{algorithm}{0}
\begin{algorithm}[H]
\caption{Two Pointers And Reverse}
\begin{algorithmic}[1]
\Procedure{ReorderList}{$H$}
\If{$H=\texttt{null}$ \textbf{or} $H.\texttt{next}=\texttt{null}$}
\State \Return
\EndIf
\State $F:=H$ and $S:=H$ \Comment Fast and Slow pointers
\While{$F.\texttt{next}\neq\texttt{null}$ \textbf{and} $F.\texttt{next}.\texttt{next}\neq\texttt{null}$}
\State $F\gets F.\texttt{next}$
\State $F\gets F.\texttt{next}$
\State $S\gets S.\texttt{next}$
\EndWhile
\State $\alpha:=S.\texttt{next}$
\State $S.\texttt{next}\gets\texttt{null}$ \Comment Break the original list
\State $\beta:=\texttt{null}$
\While{$\alpha\neq\texttt{null}$} \Comment Reverse the right hand list
\State $z:=\alpha.\texttt{next}$ \Comment Save the next node of $\alpha$
\State $\alpha.\texttt{next}\gets \beta$
\State $\beta\gets\alpha$ 
\State $\alpha\gets z$ \Comment Move $\alpha$ to next node
\EndWhile
\State $n_1:=H$ and $n_2:=\beta$ \Comment The start node of two lists
\While{$n_1\neq\texttt{null}$ \textbf{and} $n_2\neq\texttt{null}$}
\State $z_1:=n_1.\texttt{next}$
\State $n_1.\texttt{next}\gets n_2$ \Comment Set next pointer of $n_1$ to point to $n_2$
\State $z_2:=n_2.\texttt{next}$
\State $n_2.\texttt{next}\gets z_1$ \Comment Set next pointer of $n_1$ to point to next node of $n_1$
\State $n_1\gets z_1$ \Comment Move $n_1$ to its next node in original list
\State $n_2\gets z_2$ \Comment Move $n_2$ to its next node in the reversed list
\EndWhile
\EndProcedure
\end{algorithmic}
\end{algorithm}