\section{44 --- Wildcard Matching}
Given an input string ($s$) and a pattern ($p$), implement wildcard pattern matching with support for $?$ and $\ast$.

\begin{itemize}
\item $?$ Matches any single character.
\item $\ast$ Matches any sequence of characters (including the empty sequence).
\item The matching should cover the entire input string (not partial).
\end{itemize}

\paragraph{Note:}

\begin{itemize}
\item $s$ could be empty and contains only lowercase letters $a--z$.
\item $p$ could be empty and contains only lowercase letters $a--z$, and characters like $?$ or $\ast$.
\end{itemize}

\paragraph{Example 1:}

\begin{flushleft}
\textbf{Input}: $s = \texttt{aa}$, $p = a$

\textbf{Output}: \texttt{false}

\textbf{Explanation}: $a$ does not match the entire string \texttt{aa}.
\end{flushleft}

\paragraph{Example 2:}

\begin{flushleft}
\textbf{Input}: $s = \texttt{aa}$, $p = \ast$

\textbf{Output}: \texttt{true}

\textbf{Explanation}: $\ast$ matches any sequence.
\end{flushleft}


\paragraph{Example 3:}

\begin{flushleft}
\textbf{Input}: $s = \texttt{cb}$, $p = ?a$

\textbf{Output}: \texttt{false}

\textbf{Explanation}: $?$ matches $c$, but the second letter is $a$, which does not match $b$.
\end{flushleft}


\paragraph{Example 4:}

\begin{flushleft}
\textbf{Input}: $s = \texttt{adceb}$, $p = \ast a\ast b$

\textbf{Output}: \texttt{true}

\textbf{Explanation}: The first $\ast$ matches the empty sequence, while the second $\ast$ matches the substring \texttt{dce}.

\end{flushleft}

\paragraph{Example 5:}

\begin{flushleft}
\textbf{Input}: $s = \texttt{acdcb}$, $p = a\ast c?b$

\textbf{Output}: \texttt{false}
\end{flushleft}

\subsection{Dynamic Programming}
\begin{itemize}
\item Define $F(i,j)$ as the match result of $s[0, i-1]$ with $p[0, j-1]$.
\item First, we need to fill the base cases, i.e. $F(0,i)$ for $i \in [0, m]$. This means when $s$ is empty, what is the match results of a empty string with $p[0, i-1]$. Apparently, only when $p[i-1] = \ast$, it may get result of true.
\item Then, starting the fill process. There will be two cases
\begin{enumerate}
\item if $p[j-1]=\ast$, $F(i,j) = F(i-1, j)$ \textbf{or} $F(i,j-1)$, i.e., either match $\ast$ with $s[i-1]$ (then the result will be coming from the match result of $s[0, i-2]$ with $p[0, j-1]$) or treat $\ast$ as nothing (then the result will be coming from the match result of $s[0,i-1]$ with $p[0,j-2]$)
\item if $p[j-1] = s[i-1]$ \textbf{or} $p[j-1] = ?$, $F(i,j) = F(i-1,j-1)$ (i.e the result will be coming from the match result of $s[0,i-2]$ and $p[0,j-2]$)
\end{enumerate}
\end{itemize}

\setcounter{algorithm}{0}
\begin{algorithm}[H]
\caption{Dynamic Programming}
\begin{algorithmic}[1]
\Procedure{IsMatch}{$S, n, P, m$}
\State $\star$ Create $F$ as an array filled zeros with size $(n+1)\times (m+1)$
\State $F[0][0]\gets 1$ \Comment empty string $s$ matches empty string $p$
\For{$i:=1$ \textbf{to} $m$}
\If{$P[i-1] = \ast$} \Comment Only $\ast$ can matches empty string $s$
\State $F[0][i] = F[0][i-1]$
\EndIf
\EndFor
\For{$i:=1$ \textbf{to} $n$}
\For{$j:=1$ \textbf{to} $m$}
\If{$P[j-1] = \ast$}
\State $F[i][j] = F[i-1][j]$ \textbf{or} $F[i][j-1]$
\ElsIf{$P[j-1] = ?$ \textbf{or} $S[i-1] = P[j-1]$}
\State $F[i][j] = F[i-1][j-1]$
\algstore{44algo}
\end{algorithmic}
\end{algorithm}
\begin{algorithm}[H]
\begin{algorithmic}[1]
\algrestore{44algo}
\EndIf
\EndFor
\EndFor
\If{$F[n][m] = 1$}
\State \Return \textbf{true} \Comment Matched
\Else
\State \Return \textbf{false} \Comment Not matched
\EndIf
\EndProcedure
\end{algorithmic}
\end{algorithm}

\setcounter{lstlisting}{0}
\begin{lstlisting}[style=customc, caption={Dynamic Programming}]
bool isMatch( string s, string p )
{
    auto m = s.size();
    auto n = p.size();

    vector<vector<int>> F( m + 1, vector<int>( n + 1, 0 ) );

    F[0][0] = 1; //empty vs empty

    for( size_t j = 1; j <= n; ++j )
    {
        if( p[j - 1] == '*' )
        {
            //only * can match empty string
            F[0][j] = F[0][j - 1];
        }
    }

    for( size_t i = 1; i <= m; ++i )
    {
        for( size_t j = 1; j <= n; ++j )
        {
            if( p[j - 1] == '*' )
            {
                //either treat * as s[i-1]
                F[i][j] = F[i - 1][j];
                //or treat * as nothing
                F[i][j] |= F[i][j - 1];
            }
            else if( ( p[j - 1] == '?' ) || ( p[j - 1] == s[i - 1] ) )
            {
                F[i][j] = F[i - 1][j - 1];
            }
        }
    }

    return F[m][n] == 1;
}
\end{lstlisting}